new solutions

dafny-tutorial/ex12.dfy
@@ -3,5 +3,5 @@
 predicate sorted(a: array<int>)
   reads a
 {
-  false // Fill in a new body here.
+  forall j, k :: 0 <= j < k < a.Length ==> a[j] < a[k]
 }
