dafny-tutorial/ex13.dfy
@@ -1,9 +1,10 @@
 //Exercise 13. Change the definition of sorted so that it allows its argument to be null (using a nullable array type) but returns false if it is.
 
-predicate sorted(a: array<int>) // Change the type
+predicate sorted(a: array?<int>) 
   reads a
 {
-  // Change this definition to treat null arrays as "not sorted".
-  // (i.e. return false for null arrays)
-  forall j, k :: 0 <= j < k < a.Length ==> a[j] <= a[k]
+  if a==null then 
+    false 
+  else 
+    forall j, k :: 0 <= j < k < a.Length ==> a[j] <= a[k]
 }
