dafny-tutorial/ex0.dfy
@@ -2,6 +2,16 @@
 
 method Max(a: int, b: int) returns (c: int)
   // What postcondition should go here, so that the function operates as expected?
+  ensures (a == c || b == c) 
+  ensures (a <= c && b <= c)
+
+  //this one also works
+  // ensures a < b ==> c==b
+  // ensures a >= b ==> c==a
 {
-  // fill in the code here
+  if (a < b) {
+    return b;
+  } else {
+    return a;
+  }
 }
