dafny-tutorial/ex1.dfy
@@ -1,8 +1,13 @@
 //Exercise 1. Write a test method that calls your Max method from Exercise 0 and then asserts something about the result.
 
-method Max(a: int, b:int) returns (c: int)
-  // Use your code from Exercise 0
+include "ex0.dfy"
+
 method Testing() {
   // Assert some things about Max. Does it operate as you expect?
   // If it does not, can you think of a way to fix it?
+  var m := Max(0,2);
+  assert m == 2;
+
+  var m1 := Max(1,1);
+  assert m1 == 1;
 }
