dafny-tutorial/ex11.dfy
@@ -1,8 +1,20 @@
 //Exercise 11. Write a method that takes an integer array, which it requires to have at least one element, and returns an index to the maximum of the array’s elements. Annotate the method with pre- and postconditions that state the intent of the method, and annotate its body with loop invariant to verify it.
 
 method FindMax(a: array<int>) returns (i: int)
-  // Annotate this method with pre- and postconditions
-  // that ensure it behaves as described.
+  requires 0 < a.Length 
+  ensures 0 <= i < a.Length 
+  ensures forall k :: 0 <= k < a.Length ==> a[k] <= a[i]
 {
-  // Fill in the body that calculates the INDEX of the maximum.
+  i := 0;
+  var index: int := 1; 
+  while index != a.Length 
+    invariant 1 <= index <= a.Length 
+    invariant 0 <= i < index
+    invariant forall k :: 0 <= k < index ==> a[k] <= a[i]
+  {
+    if a[i] < a[index] {
+      i := index;
+    } 
+    index := index + 1;
+  }
 }
