dafny-tutorial/ex2.dfy
@@ -2,14 +2,12 @@
 
 method Abs(x: int) returns (y: int)
   // Add a precondition here.
+  requires x < 0
+
   ensures 0 <= y
   ensures 0 <= x ==> y == x
   ensures x < 0 ==> y == -x
 {
   // Simplify the body to just one return statement
-  if x < 0 {
-    return -x;
-  } else {
-    return x;
-  }
+  return -x;
 }
