dafny-tutorial/ex6.dfy
@@ -4,9 +4,17 @@ method m(n: nat)
 {
   var i: int := 0;
   while i < n
-    invariant 0 <= i <= n  // Change this. What happens?
+    invariant 0 <= i <= n + 2 
   {
     i := i + 1;
   }
-  assert i == n;
+
+  //at the end, dafny will know that
+  //0 <= i <= n+2
+  //n <= i
+  //and we can not conclude that i == n because it can be n+1 or n+2
+  
+  //assert i == n;
+
+  assert n <= i && i <= n + 2;
 }
