dafny-tutorial/ex8.dfy
@@ -9,18 +9,16 @@ function fib(n: nat): nat
 method ComputeFib(n: nat) returns (b: nat)
   ensures b == fib(n)  // Do not change this postcondition
 {
-  // Change the method body to instead use c as described.
-  // You will need to change both the initialization and the loop.
   if n == 0 { return 0; }
   var i: int := 1;
-  var a := 0;
   b := 1;
+  var c := 1;
   while i < n
     invariant 0 < i <= n
-    invariant a == fib(i - 1)
+    invariant c == fib(i + 1)
     invariant b == fib(i)
   {
-    a, b := b, a + b;
+    b, c := c, b + c;
     i := i + 1;
   }
 }
